safechecker/theories/PCUICWfEnvImpl.v
@@ -46,25 +46,6 @@ destruct (wf_ext_gc_of_uctx HΣ) as [uctx Huctx].
 exists (make_graph uctx). unfold is_graph_of_uctx. now rewrite Huctx.
 Defined.
 
-Require Import Morphisms.
-
-Global Instance consistent_proper : Proper (CS.Equal ==> iff) consistent.
-Proof.
-  intros c c' eq. rewrite /consistent.
-  now setoid_rewrite eq.
-Qed.
-
-Lemma on_udecl_mono {cf:checker_flags} {Σ : global_env} {wfΣ : wf Σ} : on_udecl Σ Monomorphic_ctx.
-Proof.
-  repeat split; cbn.
-  - intros i; rewrite LevelSetFact.empty_iff //.
-  - intros i; rewrite ConstraintSetFact.empty_iff //.
-  - red. rewrite /univs_ext_constraints /=.
-    rewrite CS_union_empty.
-    apply wfΣ.
-  - apply consistent_extension_on_empty.
-Qed.
-
 Class abstract_guard_impl :=
   { guard_impl : FixCoFix -> global_env_ext -> context -> mfixpoint term -> bool ;
     guard_correct : forall fix_cofix Σ Γ mfix, guard fix_cofix Σ Γ mfix <-> guard_impl fix_cofix Σ Γ mfix
@@ -86,18 +67,6 @@ Record referenced_impl {cf:checker_flags} := {
       referenced_impl_graph := projT1 (graph_of_wf referenced_impl_wf);
       referenced_impl_graph_wf := projT2 (graph_of_wf referenced_impl_wf)
   }.
-
-Definition init_env : global_env :=
-   {| universes := (LS.singleton Level.lzero , CS.empty); declarations := []; retroknowledge := Retroknowledge.empty |}.
-
-Definition on_global_univ_init_env : on_global_univs init_env.
-  repeat split.
-  - intros x Hx; cbn in *. inversion Hx.
-  - intros x Hx; cbn in *. destruct x; eauto. now inversion Hx.
-  - red. unshelve eexists.
-    + econstructor; eauto. intros; exact 1%positive.
-    + red. intros ? ?. cbn in *. inversion H.
-Qed.
 
 Definition check_conv_pb_relb_correct {cf:checker_flags} (Σ : global_env_ext) (HΣ : ∥ wf_ext Σ ∥) G
   (HG : is_graph_of_uctx G (global_ext_uctx Σ)) conv_pb u u' :
@@ -150,17 +119,12 @@ Program Global Instance canonical_abstract_env_struct {cf:checker_flags} {guard 
 
      abstract_env_guard := fun Σ fix_cofix => guard_impl fix_cofix (referenced_impl_env_ext Σ);
      abstract_env_ext_rel := fun X Σ => Σ = referenced_impl_env_ext X;
-     abstract_env_empty := {|
-       referenced_impl_env := {| universes := init_env ; declarations := []; retroknowledge := Retroknowledge.empty |};
- |} ;
  abstract_env_init := fun cs retro H =>  {|
  referenced_impl_env := {| universes := cs ; declarations := []; retroknowledge := retro |};
  |} ;
  abstract_env_add_decl := fun X kn d H =>
   {| referenced_impl_env := add_global_decl X.(referenced_impl_env) (kn,d);
    |};
- abstract_env_empty_ext X := {| referenced_impl_env_ext := (X , Monomorphic_ctx);
- |} ;
  abstract_env_is_consistent uctx := wGraph.is_acyclic (make_graph uctx);
  abstract_env_is_consistent_uctx X uctx :=
    let G := referenced_impl_graph X in
@@ -172,15 +136,11 @@ Program Global Instance canonical_abstract_env_struct {cf:checker_flags} {guard 
  abstract_env_rel := fun X Σ => Σ = referenced_impl_env X ;
  abstract_pop_decls := referenced_pop ;
  |}.
-Next Obligation. sq. constructor; cbn; eauto. apply on_global_univ_init_env. econstructor. Qed.
 Next Obligation. sq; constructor; cbn; eauto. econstructor. Qed.
 Next Obligation.
  pose proof (referenced_impl_wf X). destruct (H _ eq_refl).
  sq. destruct H0.  econstructor; eauto. econstructor; eauto.
   Qed.
-Next Obligation. pose proof (referenced_impl_wf X) as [?]. sq. split; eauto.
-  apply on_udecl_mono.
-Qed.
 Next Obligation.
   pose proof (referenced_impl_wf X). destruct (Hglobal _ eq_refl); sq.
   now econstructor.
@@ -225,12 +185,6 @@ Proof.
   unfold EnvMap.of_global_env. simpl. unfold KernameMapFact.uncurry.
   reflexivity.
 Qed.
-
-Program Definition wf_env_empty {cf:checker_flags} {guard : abstract_guard_impl} :=
- {|
-  wf_env_referenced := abstract_env_empty ;
-  wf_env_map := EnvMap.empty;
-  |}.
 
 Program Definition wf_env_init {cf:checker_flags} {guard : abstract_guard_impl} cs retro :
   on_global_univs cs -> wf_env := fun H =>
@@ -295,14 +249,10 @@ Program Global Instance optimized_abstract_env_struct {cf:checker_flags} {guard 
  abstract_env_guard := fun Σ fix_cofix => guard_impl fix_cofix (wf_env_ext_referenced Σ);
  abstract_env_ext_rel X := abstract_env_ext_rel X.(wf_env_ext_referenced);
 
- abstract_env_empty := wf_env_empty;
  abstract_env_init := wf_env_init;
  abstract_env_add_decl X kn d H :=
   {| wf_env_referenced := @abstract_env_add_decl _ _ referenced_impl_ext _ X.(wf_env_referenced) kn d H ;
      wf_env_map := EnvMap.add kn d X.(wf_env_map) |};
- abstract_env_empty_ext X :=
-  {| wf_env_ext_referenced := @abstract_env_empty_ext _ _ referenced_impl_ext _ X.(wf_env_referenced) ;
-     wf_env_ext_map := X.(wf_env_map) |};
  abstract_env_is_consistent univ := abstract_env_is_consistent univ;
  abstract_env_is_consistent_uctx X uctx := abstract_env_is_consistent_uctx X.(wf_env_referenced) uctx;
  abstract_env_add_udecl X udecl Hdecl :=
@@ -319,7 +269,6 @@ Next Obligation.
   destruct X1; eauto. 
   apply wf_env_map_repr.
 Qed.
-Next Obligation. apply wf_env_map_repr. Qed.
 Next Obligation. apply wf_env_map_repr. Qed.
 
 Section WfEnv.
@@ -451,7 +400,6 @@ Next Obligation. apply guard_correct. Qed.
 Next Obligation. now sq. Qed.
 Next Obligation. wf_env. Qed.
 Next Obligation. now split. Qed.
-Next Obligation. now split. Qed.
 Next Obligation. unshelve epose proof (is_consistent_spec udecl _) as Hconsistent; eauto.
   unfold is_consistent in Hconsistent; now rewrite H0 in Hconsistent.
   Qed.
@@ -488,7 +436,6 @@ Program Global Instance optimized_abstract_env_prop {cf:checker_flags} {guard : 
   Next Obligation. eapply guard_correct. Qed.
   Next Obligation. now sq. Qed.
 Next Obligation. wf_env. Qed.
-Next Obligation. now split. Qed.
 Next Obligation. now split. Qed.
 Next Obligation. now erewrite (@abstract_env_is_consistent_correct _ _ _ _ canonical_abstract_env_prop); eauto. Qed.
 Next Obligation. now erewrite (abstract_env_is_consistent_uctx_correct X.(wf_env_referenced)); eauto. Qed.
